cfi/cfi_refinementAS.v
@@ -1,0 +1,172 @@
+Require Import cfi.cfi_refinement.
+Require Import cfi.abstract.
+Require Import cfi.symbolic.
+Require Import cfi.refinementAS.
+Require Import cfi.cfi_rules.
+Require Import symbolic.symbolic.
+Require Import common.common.
+Require Import lib.utils.
+Require Import lib.partial_maps.
+Require Import lib.Coqlib.
+
+Require Import ssreflect ssrfun ssrbool eqtype ssrnat seq.
+
+Set Implicit Arguments.
+
+Import PartMaps.
+ 
+Section Refinement.
+
+Context {t : machine_types}
+        {ops : machine_ops t}
+        {opss : machine_ops_spec ops}
+        
+        {ap : Abstract.abstract_params t}
+        {aps : Abstract.params_spec ap}
+
+        {smemory : Type}
+        {sm : partial_map smemory (word t) (atom (word t) (@cfi_tag t))}
+        {smems : axioms sm}
+        {smemory_map : Map.mappable sm (@Abstract.dmem_class t ap)}
+        {smemory_filter : Filter.filterable sm}
+
+        {sregisters : Type}
+        {sr : partial_map sregisters (reg t) (atom (word t) (@cfi_tag t))}
+        {sregs : axioms sr}
+        {sregs_map : Map.mappable sr (@Abstract.reg_class t ap)}.
+
+Variable valid_jmp : word t -> word t -> bool.
+
+Definition sym_params := SymbolicCFI.sym_cfi valid_jmp.
+
+Variable atable : list (Abstract.syscall t).
+Variable stable : list (@Symbolic.syscall t sym_params).
+
+Definition amachine :=  Abstract.abstract_cfi_machine atable valid_jmp.
+Definition smachine := SymbolicCFI.symbolic_cfi_machine stable.
+
+Program Instance cfi_refinementAS  : 
+  (@machine_refinement t amachine smachine) := {
+    refine_state st st' := RefinementAS.refine_state st st';
+
+    visible st st' := true
+}.
+Next Obligation.
+  split; 
+  [intros; destruct (RefinementAS.backwards_simulation atable ast REF STEP) 
+    as [? [? ?]];
+   eexists; split; eauto | discriminate].
+Qed.
+Next Obligation.
+  destruct (RefinementAS.backwards_simulation_attacker ast REF STEPA);
+  eexists; eauto.
+Qed.
+  
+Definition astop (xs : list (@cfi.state t amachine)) := Abstract.S atable valid_jmp xs.
+
+Definition sstop (xs : list (@cfi.state t smachine)) := 
+  SymbolicCFI.S stable xs.
+
+Hypothesis refine_syscalls_correct : RefinementAS.refine_syscalls atable stable.
+
+Ltac match_inv :=
+  repeat match goal with
+  | H : bind (fun x : _ => _) _ = Some _ |- _ =>
+    apply bind_inv in H;
+    let x := fresh x in
+    let E := fresh "E" in
+    destruct H as (x & H & E);
+    simpl in H; simpl in E
+  | H : (if ?b then _ else _) = Some _ |- _ =>
+    let E := fresh "E" in
+    destruct b eqn:E;
+    try discriminate
+  | H : match ?E with _ => _ end = _ |- _ =>
+    destruct E eqn:?; try discriminate
+  | H : Some _ = Some _ |- _ => inv H
+  | H : ?O = Some _ |- context[bind _ ?O] => rewrite H; simpl
+  | H : True |- _ => clear H
+  end.
+
+Program Instance cfi_refinementAS_specs :
+  machine_refinement_specs astop sstop cfi_refinementAS.
+Next Obligation. (*step or no step*)
+  Admitted.
+Next Obligation. (*initial state*)
+  Admitted.
+Next Obligation.
+  destruct asi as [[[[imem dmem] aregs] apc] b], 
+           asj as [[[[imem' dmem'] aregs'] apc'] b'].
+  destruct csi as [mem regs [spc tpc] int].
+  destruct csj as [mem' regs' [spc' tpc'] int'].
+  destruct H as [REFI [REFD [REFR [REFPC CORRECTNESS]]]].
+  destruct H0 as [REFI' [REFD' [REFR' [REFPC' CORRECTNESS']]]].
+  unfold Abstract.succ in H1.
+  unfold RefinementAS.refine_pc in REFPC; simpl in REFPC; 
+  destruct REFPC as [? TPC];
+  unfold RefinementAS.refine_pc in REFPC'; simpl in REFPC'; 
+  destruct REFPC' as [? TPC'];
+  subst.
+  unfold SymbolicCFI.ssucc; simpl.
+  destruct (get imem spc) eqn:GET.
+  + destruct (decode_instr s) eqn:INST.
+    - destruct i eqn:DECODE;
+      apply REFI in GET;
+      destruct GET as [id GET'];
+      rewrite GET'; simpl;
+      rewrite INST; try assumption. 
+      (*syscall case*)
+  (* + discriminate. *)
+Admitted.
+Next Obligation.
+  assert (ST := Abstract.step_succ_violation H H0).
+  intro CONTRA.
+  destruct CONTRA. discriminate.
+Qed.
+Next Obligation.
+  unfold Abstract.succ in H1.
+  destruct ast as [[[[imem dmem] aregs] apc] b],
+           ast' as [[[[imem' dmem'] aregs'] apc'] b'].
+  destruct cst as [mem reg [pc tpc] int].
+  destruct cst' as [mem' reg' [pc' tpc'] int'].
+  destruct H as [REFI [REFD [REFR [REFPC CORRECT]]]],
+           H0 as [REFI' [REFD' [REFR' [REFPC' CORRECT']]]].
+  unfold RefinementAS.refine_pc in *.
+  simpl in REFPC; simpl in REFPC'; destruct REFPC as [? TPC],
+                                            REFPC' as [? TPC'].
+  subst.
+  unfold SymbolicCFI.ssucc.    
+  destruct (get imem pc) eqn:GET.
+  { apply REFI in GET.
+    destruct GET as [id GET].
+    destruct (decode_instr s) eqn:INST.
+    { destruct i;
+      simpl; rewrite GET; simpl; rewrite INST; auto. 
+    }
+    { simpl. rewrite GET. rewrite INST. assumption. }
+  }
+  { destruct (Abstract.get_syscall atable pc) eqn:GETCALL.
+    { discriminate. }
+    { simpl. 
+      destruct (get mem pc) eqn:GET'.
+      { destruct a. destruct tag.
+        { assert (EGET' : exists id, get mem pc = Some val@(INSTR id)) 
+               by (eexists; eauto). 
+          apply REFI in EGET'. congruence.
+        }
+        { rewrite GET'. reflexivity. } 
+      } rewrite GET'. reflexivity. }
+  }
+Qed.
+Next Obligation.
+  unfold astop in H0. unfold Abstract.S in H0.
+  unfold sstop. unfold SymbolicCFI.S.
+  destruct H0 as [s [EQ NOSTEP]].
+  inversion EQ; subst.
+  inversion H; subst.
+  - exists cst. split; auto.
+    intro CONTRA. destruct CONTRA as [s' CONTRA].
+    destruct (backwards_refinement_normal _ _ _ H2 CONTRA).
+Admitted. (*stuck?*)
+        
+End Refinement.
